cava/cava/Cava/Signal.v
@@ -1,0 +1,26 @@
+(****************************************************************************)
+(* Copyright 2020 The Project Oak Authors                                   *)
+(*                                                                          *)
+(* Licensed under the Apache License, Version 2.0 (the "License")           *)
+(* you may not use this file except in compliance with the License.         *)
+(* You may obtain a copy of the License at                                  *)
+(*                                                                          *)
+(*     http://www.apache.org/licenses/LICENSE-2.0                           *)
+(*                                                                          *)
+(* Unless required by applicable law or agreed to in writing, software      *)
+(* distributed under the License is distributed on an "AS IS" BASIS,        *)
+(* WITHOUT WARRANTIES OR CONDITIONS OF ANY KIND, either express or implied. *)
+(* See the License for the specific language governing permissions and      *)
+(* limitations under the License.                                           *)
+(****************************************************************************)
+
+From Coq Require Import Ascii String.
+From Coq Require Import ZArith.
+
+Inductive Signal : Type :=
+  | Gnd: Signal
+  | Vcc: Signal
+  | Wire: N -> Signal
+  | NamedWire: string -> Signal
+  | NamedBitVec: string -> list nat -> Signal
+  | Vec: list Signal -> Signal.
